\documentclass{article}
\usepackage{backnaur}
\usepackage{amsmath}

\begin{document}
\section{Operational Semantics}
\subsection{Notation}
The state of the evaluator, $\sigma$, consists of a \\
packet, $\pi$\\
action\_list, $\alpha$ \\
stored\_action\_list, $\Lambda$ \\
context, $\xi$, which is the tuple: \\
$[ ingress\_port, \ egress\_port, \ physical\_port, \ key, \ meta, \ header\_offset, \ table ]$
\\ \\
$\pi$ can be introspected with angle brackets, $\langle \ \rangle$ \\
$\xi$ can be introspected with square brackets, $\lbrack \ \rbrack$ \\
$\alpha$ can be introspected with parentheses, ( ) \\
$\Lambda$ can be introspected with $\Lambda$ following parenthesis, $\Lambda$( ) \\
$\sigma$ can be introspected with curly braces, \{ \} \\
\subsection{Operational Semantics 5-Tuple}
$ pip = \langle IF, \ CF, \ \Rightarrow, \ FC, \ OF \rangle $\\
IF = $program \times \pi \rightarrow CF$ \\
CF = $\alpha \times \xi \times \pi$ \\
$\Rightarrow$ = Defined in section ``Reduction Relation''. \\
FC = $\pi \times \xi$ \\
OF = $FC \rightarrow \textrm{serialization}$

\subsection{Reduction Relation}
\begin{equation}
  (\textbf{\textrm{advance}} \ n)\textrm{,} \ [header\_offset], \ \bar \alpha \Rightarrow [header\_offset + n], \ \bar \alpha'
\end{equation}

\begin{equation}
  (\textrm{\textbf{clear}}) \textrm{,} \ \Lambda \Rightarrow \Lambda()
\end{equation}

\begin{equation}
  (\textrm{\textbf{drop})} \textrm{,} \ \sigma \Rightarrow \{ \}
\end{equation}

\begin{equation}
  (\textrm{\textbf{write}} \ action), \ \Lambda \Rightarrow \Lambda \cdot action
\end{equation}

\begin{equation}
  (\textrm{\textbf{goto}} \ table_t) \textrm{,} \ [table] \Rightarrow
  [table_t]
\end{equation}

\begin{equation}
  (\textrm{\textbf{set}} \ field \ value) \Rightarrow \langle field = value \rangle
\end{equation}

\begin{equation}
  (\textrm{\textbf{output}} \ port) \textrm{,} \ [egress\_port] \Rightarrow
  [egress\_port = port]
\end{equation}

\begin{equation}
\begin{split}
  (\textrm{\textbf{copy}} \ as_1 \ src \ as_2 \ dst \ n) \Rightarrow \langle
  dst \rangle = [[meta, meta + n)] \\ 
    \textrm{where} \ as_1 = \textrm{\textbf{meta} and } as_2 =
    \textrm{\textbf{packet}}
\end{split}
\end{equation}

\begin{equation}
\begin{split}
  (\textrm{\textbf{copy}} \ as_1 \ src \ as_2 \ dst \ n) \Rightarrow \langle
  dst + [header\_offset] \rangle = \\
  [[meta, meta + n)] \\ 
    \textrm{where} \ as_1 = \textrm{\textbf{meta} and } as_2 =
    \textrm{\textbf{header}}
\end{split}
\end{equation}

\begin{equation}
\begin{split}
  (\textrm{\textbf{copy}} \ as_1 \ src \ as_2 \ dst \ n) \Rightarrow [key] =
  [[meta, meta + n)] \\ 
    \textrm{where} \ as_1 = \textrm{\textbf{meta} and } as_2 =
    \textrm{\textbf{key}}
\end{split}
\end{equation}

\begin{equation}
\begin{split}
  (\textrm{\textbf{copy}} \ as_1 \ src \ as_2 \ dst \ n) \Rightarrow \langle
  dst + [header\_offset] \rangle = [[meta, meta + n)] \\ 
    \textrm{where} \ as_1 = \textrm{\textbf{meta} and } as_2 =
    \textrm{\textbf{header}}
\end{split}
\end{equation}

\begin{equation}
\begin{split}
  (\textrm{\textbf{copy}} \ as_1 \ src \ as_2 \ dst \ n) \Rightarrow \langle
  dst \rangle = \langle [src, src + n) \rangle \\ 
    \textrm{where} \ as_1 = \textrm{\textbf{packet} and } as_2 =
    \textrm{\textbf{packet}}
\end{split}
\end{equation}

\begin{equation}
\begin{split}
  (\textrm{\textbf{copy}} \ as_1 \ src \ as_2 \ dst \ n) \Rightarrow \langle
  dst + [header\_offset] \rangle =  \langle [src, src + n) \rangle \\ 
    \textrm{where} \ as_1 = \textrm{\textbf{packet} and } as_2 =
    \textrm{\textbf{header}}
\end{split}
\end{equation}

\begin{equation}
\begin{split}
  (\textrm{\textbf{copy}} \ as_1 \ src \ as_2 \ dst \ n) \Rightarrow [key] =
  \langle [src, src + n) \rangle \\ 
    \textrm{where} \ as_1 = \textrm{\textbf{packet} and } as_2 =
    \textrm{\textbf{key}}
\end{split}
\end{equation}

\begin{equation}
\begin{split}
  (\textrm{\textbf{copy}} \ as_1 \ src \ as_2 \ dst \ n) \Rightarrow \langle
  dst + [header\_offset] \rangle = \\
  \langle [src + [header\_offset], src + [header\_offset] + n) \rangle \\ 
    \textrm{where} \ as_1 = \textrm{\textbf{header} and } as_2 =
    \textrm{\textbf{header}}
\end{split}
\end{equation}

\begin{equation}
\begin{split}
  (\textrm{\textbf{copy}} \ as_1 \ src \ as_2 \ dst \ n) \Rightarrow \langle
  dst \rangle = \\
  \langle [src + [header\_offset], src + [header\_offset] + n) \rangle \\ 
    \textrm{where} \ as_1 = \textrm{\textbf{header} and } as_2 =
    \textrm{\textbf{packet}}
\end{split}
\end{equation}

\begin{equation}
\begin{split}
  (\textrm{\textbf{copy}} \ as_1 \ src \ as_2 \ dst \ n) \Rightarrow [key] = \\
  \langle [src + [header\_offset], src + [header\_offset] + n) \rangle \\ 
    \textrm{where} \ as_1 = \textrm{\textbf{header} and } as_2 =
    \textrm{\textbf{key}}
\end{split}
\end{equation}

\begin{equation}
\begin{split}
  (\textrm{\textbf{copy}} \ as_1 \ src \ as_2 \ dst \ n) \Rightarrow [meta] = \\
  \langle [src + [header\_offset], src + [header\_offset] + n) \rangle \\ 
    \textrm{where} \ as_1 = \textrm{\textbf{header} and } as_2 =
    \textrm{\textbf{meta}}
\end{split}
\end{equation}

\end{document}
